theories/examples/enclaves/trusted_compute_adequacy.v
@@ -10,6 +10,7 @@ From iris.proofmode Require Import proofmode.
 From cap_machine Require Import rules logrel fundamental.
 From cap_machine Require Import proofmode.
 From cap_machine Require Import assert macros_new.
+From cap_machine Require Import attestation_adequacy_template.
 From cap_machine Require Import
   trusted_compute_code
   trusted_compute_enclave_spec
@@ -20,6 +21,7 @@ From cap_machine Require Import
 (* Instance DisjointList_list_Addr : DisjointList (list Addr). *)
 (* Proof. exact (@disjoint_list_default _ _ app []). Defined. *)
 
+Import assert_lib.
 Class memory_layout `{MachineParameters} := {
   (* Verifier code *)
   verifier_region_start : Addr;
@@ -68,6 +70,11 @@ Class memory_layout `{MachineParameters} := {
   link_table_region_correct:
     link_table_region = (finz.seq_between l_assert_start l_assert_end);
 
+  (* TC enclave *)
+  tc_enclave_start : Addr;
+  tc_enclave_end : Addr;
+  tc_enclave_size : (tc_enclave_start + (length trusted_compute_enclave_instrs + 1))%a =  Some tc_enclave_end;
+
   regions_disjoints :
   verifier_region ## adv_region ∧
   verifier_region ## l_assert_region ∧
@@ -77,58 +84,52 @@ Class memory_layout `{MachineParameters} := {
   l_assert_region ## link_table_region;
 }.
 
-(* Definition tc_verifier_prog `{memory_layout} : prog := *)
-(*   {| prog_start := verifier_start ; *)
-(*      prog_end := verifier_end ; *)
-(*      prog_instrs := trusted_compute_main_code 0 ; *)
-(*      prog_size := verifier_size |}. *)
+Local Instance trusted_compute_concrete `{memory_layout} : TrustedCompute.
+Proof. apply (Build_TrustedCompute tc_enclave_start). Defined.
 
-(* Definition adv_prog `{memory_layout} : prog := *)
-(*   {| prog_start := adv_start ; *)
-(*      prog_end := adv_end ; *)
-(*      prog_instrs := adv_instrs ; *)
-(*      prog_size := adv_size |}. *)
+Program Definition tc_verifier_prog `{memory_layout} : prog :=
+  let link_cap := WCap RO link_table_start link_table_end link_table_start in
+  let a_data := (verifier_start ^+ trusted_compute_main_code_len)%a in
+  let data_cap := WCap RWX verifier_start verifier_end a_data  in
+  {| prog_start := verifier_start ;
+     prog_end := verifier_end ;
+     prog_instrs :=
+      (lword_get_word <$> (trusted_compute_main_code 0))
+       ++ [link_cap ; data_cap];
+     prog_size := _ |}.
+Next Obligation.
+  intros MP ML *.
+  rewrite -verifier_size.
+  rewrite app_length.
+  rewrite fmap_length.
+  by cbn.
+Qed.
 
-(* Program Definition layout `{memory_layout} : ocpl_library := *)
-(*   {| (* malloc library *) *)
-(*      malloc_start := l_malloc_start; *)
-(*      malloc_memptr := l_malloc_memptr; *)
-(*      malloc_mem_start := l_malloc_mem_start; *)
-(*      malloc_end := l_malloc_end; *)
+Definition adv_prog `{memory_layout} : prog :=
+  {| prog_start := adv_start ;
+     prog_end := adv_end ;
+     prog_instrs := adv_instrs ;
+     prog_size := adv_size |}.
 
-(*      malloc_code_size := l_malloc_code_size; *)
+Program Definition layout `{memory_layout} : assert_library :=
+  {| (* assertion fail library *)
+     assert_start := l_assert_start;
+     assert_cap := l_assert_cap;
+     assert_flag := l_assert_flag;
+     assert_end := l_assert_end;
 
-(*      malloc_memptr_size := l_malloc_memptr_size; *)
+     assert_code_size := l_assert_code_size;
+     assert_cap_size := l_assert_cap_size;
+     assert_flag_size := l_assert_flag_size;
+  |}.
+Definition AssertLibrary `{memory_layout} := library layout.
 
-(*      malloc_mem_size := l_malloc_mem_size; *)
-
-(*      (* assertion fail library *) *)
-(*      assert_start := l_assert_start; *)
-(*      assert_cap := l_assert_cap; *)
-(*      assert_flag := l_assert_flag; *)
-(*      assert_end := l_assert_end; *)
-
-(*      assert_code_size := l_assert_code_size; *)
-(*      assert_cap_size := l_assert_cap_size; *)
-(*      assert_flag_size := l_assert_flag_size; *)
-
-(*      (* disjointness of the two libraries *) *)
-(*      libs_disjoint := _ *)
-(*   |}. *)
-(* Next Obligation. *)
-(*   intros. *)
-(*   pose proof (regions_disjoint) as Hdisjoint. *)
-(*   rewrite !disjoint_list_cons in Hdisjoint |- *. *)
-(*   set_solver. *)
-(* Qed. *)
-(* Definition OCPLLibrary `{memory_layout} := library layout. *)
-
-(* Program Definition roe_table `{memory_layout} : @tbl_priv roe_prog OCPLLibrary := *)
-(*   {| prog_lower_bound := f_region_start ; *)
+(* Program Definition tc_link_table `{memory_layout} : @tbl_priv tc_verifier_prog AssertLibrary := *)
+(*   {| prog_lower_bound := verifier_region_start ; *)
 (*      tbl_start := link_table_start ; *)
 (*      tbl_end := link_table_end ; *)
 (*      tbl_size := link_table_size ; *)
-(*      tbl_prog_link := f_region_start_offset ; *)
+(*      tbl_prog_link := verifier_region_start_offset ; *)
 (*      tbl_disj := _ *)
 (*   |}. *)
 (* Next Obligation. *)
@@ -138,7 +139,7 @@ Class memory_layout `{MachineParameters} := {
 (*   disjoint_map_to_list. set_solver. *)
 (* Qed. *)
 
-(* Program Definition adv_table `{memory_layout} : @tbl_pub adv_prog OCPLLibrary := *)
+(* Program Definition adv_table `{memory_layout} : @tbl_pub adv_prog AssertLibrary := *)
 (*   {| prog_lower_bound := adv_region_start ; *)
 (*      tbl_start := adv_link_table_start ; *)
 (*      tbl_end := adv_link_table_end ; *)
